Detailed sketcth of the Sort translation

forcing/Soundness.v
@@ -28,23 +28,30 @@ Definition leq_refl sigma t : leq_term sigma t t = true.
   induction t.
 Admitted.
 
-(** We assume the following sorts for the objects and morphisms of the base category *)
-Axiom obj_sort : forall Σ Γ, Σ ;;; Γ |- tConst "Obj" [] : tSort [Universe.Expr.set].
-Axiom hom_sort : forall Σ Γ t1 t2,
-    Σ ;;; Γ |- t1 : tConst "Obj" [] ->
-    Σ ;;; Γ |- t2 : tConst "Obj" [] ->
-                    Σ ;;; Γ |- tApp (Ast.tConst "Hom" []) [t1; t2] : tSort [Universe.Expr.set].
-Axiom id_hom_type : forall Σ Γ t,
-    Σ ;;; Γ |- t : tConst "Obj" [] ->
-    Σ ;;; Γ |- tApp (Ast.tConst "Id_hom" []) [t] : tApp (Ast.tConst "Hom" []) [t; t].
+Definition cat_obj := tConst "Obj" [].
+Definition cat_hom := tConst "Hom" [].
+Definition id_hom := tConst "Id_hom" [].
+Definition sort_set := tSort [Universe.Expr.set].
 
+(** We assume the following sorts for the objects and morphisms of the base category *)
+Axiom obj_sort : forall Σ Γ, Σ ;;; Γ |- cat_obj : sort_set.
+Axiom hom_sort : forall Σ Γ t1 t2,
+    Σ ;;; Γ |- t1 : cat_obj ->
+    Σ ;;; Γ |- t2 : cat_obj ->
+    Σ ;;; Γ |- tApp cat_hom [t1; t2] : sort_set.
+Axiom id_hom_type : forall Σ Γ t,
+    Σ ;;; Γ |- t : cat_obj ->
+    Σ ;;; Γ |- tApp id_hom [t] : tApp cat_hom [t; t].
 
 Lemma wf_init_graph : wf_graph init_graph.
 Proof.
   constructor.
   - constructor.
-    + apply SetoidList.InA_cons_tl. auto.
-    + intuition. apply SetoidList.InA_cons_hd; auto.
+    + apply SetoidList.InA_cons_tl.
+      apply SetoidList.InA_cons_hd. reflexivity.
+    + intuition. apply SetoidList.InA_cons_tl. apply SetoidList.InA_cons_tl.
+      apply SetoidList.InA_cons_hd. reflexivity.
+      apply SetoidList.InA_cons_hd; auto.
       simpl. apply SetoidList.InA_cons_hd; eauto.
       (* NOTE: something is not right, either [wf_graph] or [init_graph] *)
 Admitted.
@@ -80,16 +87,14 @@ where "E ## Γ |= σ" := (fctx_valid E Γ σ).
 Lemma last_condition_sound σ Γ (Σ := ([], init_graph)) :
   type_local_env Σ Γ ->
   (of_global_context Σ) ## Γ |= σ ->
-  Σ ;;; Γ |- tRel (last_condition σ) : tConst "Obj" [].
+  Σ ;;; Γ |- tRel (last_condition σ) : cat_obj.
 Proof.
   intros TyCtx FCvalid.
   induction FCvalid.
-  - simpl. setctx Γ'.
-         assert (H1 : 0 < #|Γ'|) by (subst;simpl; omega).
-         subst. apply type_Rel with (n:=0) (isdecl:=H1).
+  - simpl. solve_rel.
   - simpl.
     pose [vass (nNamed "t") Relevant T] as Γ'.
-    change (Σ;;; Γ ,,, Γ' |- lift0 #|Γ'| (tRel (last_condition σ)) : lift0 #|Γ'| (tConst "Obj" [])).
+    change (Σ;;; Γ ,,, Γ' |- lift0 #|Γ'| (tRel (last_condition σ)) : lift0 #|Γ'| (cat_obj)).
     assert (TyCtxΓ : type_local_env Σ Γ).
     { inversion TyCtx;subst;auto. }
     apply weakening.
@@ -115,9 +120,9 @@ Proof.
   + eapply obj_sort.
   + econstructor.
     * eapply hom_sort.
-      ** pose (vass pos_name Relevant (tConst "Obj" []) :: nil) as Γ'.
+      ** pose (vass pos_name Relevant (cat_obj) :: nil) as Γ'.
          change
-           (Σ;;; Γ ,,, Γ' |- lift0 #|Γ'| (tRel (last_condition σ)) : lift0 #|Γ'| (tConst "Obj" [])).
+           (Σ;;; Γ ,,, Γ' |- lift0 #|Γ'| (tRel (last_condition σ)) : lift0 #|Γ'| cat_obj).
          apply weakening with (Γ' := Γ').
          *** simpl. constructor. apply wf_init_graph.
          *** simpl. constructor. apply TyCtx. econstructor. simpl. apply obj_sort.
@@ -165,24 +170,58 @@ Lemma forcing_context_soundness Σ Γ σ :
   type_local_env Σ Γ -> type_local_env Σ (⟦Γ⟧ Σ σ).
 Admitted.
 
+
+Tactic Notation "solve_last_cond" :=
+  apply last_condition_sound;
+  [apply forcing_context_soundness;assumption |
+   apply context_traslation_valid;assumption].
+
+Ltac type_spine_step :=
+  match goal with
+    | [  |- typing_spine _ _ _ (?t :: ?ts) _ ] =>
+      econstructor;
+      [eapply cumul_refl;apply leq_refl | | ]
+  end.
+
+Lemma sort_translation_prefix_sound (Σ := (nil,init_graph)) σ Γ T l:
+  let E := (of_global_context Σ) in
+  let fctx := (mkFCtxt σ cat []) in
+  let srt := tSort (Universe.sup [Universe.Expr.set]  (Universe.sup [Universe.Expr.set] l)) in
+  let ext1 := get_ctx_lift cat E (last_condition σ) in
+  let ext2 := get_ctx_lift cat E (last_condition (σ ,, fcLift)) in
+  type_local_env Σ Γ ->
+  Σ ;;; Γ ,,, ext1 ,,, ext2  |- T : tSort l ->
+  Σ ;;; Γ |- snd (sort_translation_prefix E fctx tt) T
+                      : snd (Π_q_f E fctx) srt.
+Proof.
+  intros ? ? ? ? ? TyΓ TyT.
+  simpl.
+  apply lam_q_f_sound;simpl.
+  - assumption.
+  - unfold sort_set.
+    eapply Π_q_f_lift_sound. apply TyT.
+Qed.
+
 Lemma forcing_typing_soundness (Σ := (nil,init_graph)) Γ t T σ  :
   type_local_env Σ Γ ->
   Σ ;;; Γ |- t : T ->
-  let Σ' := Σ in Σ' ;;; (⟦Γ⟧ Σ σ) |- ([t]ᵗ Σ σ) : (⟦T⟧ᵀ Σ σ).
+  let Σ' := Σ in
+  Σ' ;;; (⟦Γ⟧ Σ σ) |- ([t]ᵗ Σ σ) : (⟦T⟧ᵀ Σ σ).
 Proof.
   intros TyCtx Ty.
   induction Ty; simpl.
-  - simpl. unfold translate_var.
+  - (* -- Variables -- *)
+    simpl. unfold translate_var.
     unshelve econstructor; simpl.
     Focus 2. constructor.  admit.
-  - destruct l;simpl.
-    + (* Simplifying the applications in the type first*)
-      eapply type_Conv.
-      * unfold ft_term,otranslate,lambda_prefix,extend. simpl.
-        apply lam_q_f_sound;simpl.
+  - (* -- Sorts -- *)
+    (* Simplifying the applications in the type first*)
+      unfold ft_term,otranslate,lambda_prefix,extend.
+      eapply type_Conv;simpl.
+      * apply lam_q_f_sound;simpl;auto.
         ** apply forcing_context_soundness;assumption.
         ** eapply Π_q_f_lift_sound; apply type_Sort.
-      * unfold ft_type. simpl. unfold mkOptApp.
+      * unfold ft_type. simpl in *. unfold mkOptApp.
         eapply type_App.
         ** eapply lam_q_f_sound;simpl.
            *** apply forcing_context_soundness;assumption.
@@ -191,23 +230,27 @@ Proof.
            (* TODO: show that [tSort [(Level.set, true)]] has type [tSort l] for some level l *)
            (* constructor [type_Sort] does not apply here. *)
                admit.
-        ** (* typing_spine *)
-           simpl. econstructor.
-           *** eapply cumul_refl. apply leq_refl.
-           *** apply last_condition_sound.
-               **** apply forcing_context_soundness;assumption.
-               **** apply context_traslation_valid. apply TyCtx.
-           *** econstructor.
-               **** eapply cumul_refl. apply leq_refl.
-               **** simpl. apply id_hom_type. apply last_condition_sound.
-                    ***** apply forcing_context_soundness;assumption.
-                    ***** apply context_traslation_valid. apply TyCtx.
-               **** simpl. econstructor.
+        ** simpl. (* typing_spine *)
+           type_spine_step. solve_last_cond.
+           type_spine_step. apply id_hom_type. solve_last_cond.
+           apply type_spine_nil.
       * simpl. unfold ft_type. simpl. unfold mkOptApp.
+        eapply cumul_red_r. Focus 2.
+        eapply red_beta. simpl.
+        eapply cumul_red_r. Focus 2.
+        eapply red_beta. simpl.
+        eapply cumul_refl.
+        simpl.
+        (* NOTE: not sure how to prove this stuff about [leq_universe]  *)
+        assert (H : leq_universe
+                      init_graph
+                      (Universe.sup [Universe.Expr.set]
+                                    (Universe.sup [Universe.Expr.set] (Universe.super l)))
+                      (Universe.super l) = true). admit.
+        rewrite H. rewrite Nat.eqb_refl. reflexivity.
+  - admit.
+  - (* Products *)
 
-        (* constructor. simpl. *)
-        (* apply Π_q_f_lift_sound. unfold Universe.super. simpl. *)
-        (* unfold Universe.type1,Universe.Expr.type1. *)
        (* econstructor;simpl. Focus 4. *)
        (* eapply cumul_red_r. *)
        (* Focus 2. eapply red_beta. simpl. *)
